proof/UsageExample.ec
@@ -1,0 +1,83 @@
+require import AllCore Int IntDiv List.
+
+
+from Jasmin require import JModel_x86.
+import SLH64.
+
+require JBigNumber.
+require import MLeakage.
+
+
+require Bn_util Bn_base Bn_rnd Bn_exp Fp_base Fp_mont.
+
+(* Adapt to fit the use case... *)
+
+from JExtract require import XtrCode.
+from JExtract require XtrCodeCT.
+from JExtract require import Array11 Array22 Array88 WArray88.
+
+abbrev nlimbs = 11.
+
+print XtrCode.
+
+clone import JBigNumber.BigN
+ with op nlimbs <- 11,
+      theory BN.A <= Array11,
+      theory BN2.A <= Array22,
+      theory BN_Abytes <= Array88,
+      theory BN_WAbytes <= WArray88
+      proof gt0_nlimbs by done.
+
+
+(* --- *)
+
+
+clone Fp_mont as FPM
+ with op nlimbs <- nlimbs,
+      theory BigN <- BigN,
+      op P <- bn XtrCode.glob_P,
+      op glob_P <- XtrCode.glob_P,
+      op glob_mP <- XtrCode.glob_mP,
+      op glob_P0i <- XtrCode.glob_P0i,
+      op glob_exp0 <- XtrCode.glob_exp0,
+      op glob_Pm2 <- XtrCode.glob_Pm2
+(*      theory BNUTIL <- BNUTIL,
+      theory BNB <- BNB*)
+(*      theory FPB <- FPB*)
+      proof gt0_nlimbs by done.
+
+
+equiv FPM_mulm_eq:
+ FPM.FPB.M(FPM.M.P_FP)._mulm_ ~ XtrCode.M(Syscall).fPM_mulm_ : ={arg} ==> ={res}
+by sim.
+
+equiv BN_eq_eq:
+ FPM.BNB.M._eq_ ~ XtrCode.M(Syscall).bN_eq_ : ={arg} ==> ={res}
+by sim.
+
+equiv BN_muln_eq:
+ FPM.BNB.M._muln_ ~ XtrCode.M(Syscall).bN_muln_ : ={arg} ==> ={res}
+by sim.
+
+print FPM.BNB._muln__ll.
+
+equiv BN_cswap_mask_eq:
+ FPM.BNB.M._cswap_mask_ ~ XtrCode.M(Syscall).bN_cswap_mask_ : ={arg} ==> ={res}
+by sim.
+
+equiv BN_rsample_eq:
+ FPM.FPB.BNRND.M._rsample_ ~ XtrCode.M(Syscall).bN_rsample_
+ : ={arg} ==> ={res}
+by sim.
+
+
+
+(* And now with leakage annotations... *)
+equiv BN_muln_eqLeak:
+ FPM.BNB.MLeak._muln_ ~ XtrCodeCT.M(XtrCodeCT.Syscall).bN_muln_ :
+ ={arg} /\ LEAK.leakages{1} = XtrCodeCT.M.leakages{2} 
+ ==> ={res} /\ LEAK.leakages{1} = XtrCodeCT.M.leakages{2}
+by sim.
+
+
+
