proof/extracted/XtrCodeCT.ec
@@ -1,0 +1,2441 @@
+require import AllCore IntDiv CoreMap List Distr.
+from Jasmin require import JModel_x86.
+import SLH64.
+
+from Jasmin require import JLeakage.
+require import Array3 Array11 Array22 Array88.
+require import WArray24 WArray88 WArray176.
+
+abbrev glob_rMP = Array11.of_list witness [W64.of_int 0; W64.of_int 0;
+W64.of_int 0; W64.of_int 0; W64.of_int 0; W64.of_int 0; W64.of_int 0;
+W64.of_int 0; W64.of_int 0; W64.of_int 0; W64.of_int 0].
+
+
+abbrev glob_exp0 = Array11.of_list witness [W64.of_int 0; W64.of_int 0;
+W64.of_int 0; W64.of_int 0; W64.of_int 0; W64.of_int 0; W64.of_int 0;
+W64.of_int 0; W64.of_int 0; W64.of_int 0; W64.of_int 0].
+
+
+abbrev glob_Pm2 = Array11.of_list witness [W64.of_int 0; W64.of_int 0;
+W64.of_int 0; W64.of_int 0; W64.of_int 0; W64.of_int 0; W64.of_int 0;
+W64.of_int 0; W64.of_int 0; W64.of_int 0; W64.of_int 0].
+
+
+abbrev glob_P0i = W64.of_int 0.
+
+
+abbrev glob_mP = Array11.of_list witness [W64.of_int 0; W64.of_int 0;
+W64.of_int 0; W64.of_int 0; W64.of_int 0; W64.of_int 0; W64.of_int 0;
+W64.of_int 0; W64.of_int 0; W64.of_int 0; W64.of_int 0].
+
+
+abbrev glob_P = Array11.of_list witness [W64.of_int 0; W64.of_int 0;
+W64.of_int 0; W64.of_int 0; W64.of_int 0; W64.of_int 0; W64.of_int 0;
+W64.of_int 0; W64.of_int 0; W64.of_int 0; W64.of_int 0].
+
+
+module type Syscall_t = {
+  proc randombytes_88(_:W8.t Array88.t) : W8.t Array88.t
+}.
+
+module Syscall : Syscall_t = {
+  proc randombytes_88(a:W8.t Array88.t) : W8.t Array88.t = {
+    a <$ dmap WArray88.darray
+         (fun a => Array88.init (fun i => WArray88.get8 a i));
+    return a;
+  }
+}.
+
+module M(SC:Syscall_t) = {
+  var leakages : leakages_t
+  
+  proc bN__cf_mask (cf:bool) : W64.t = {
+    var aux_0: bool;
+    var aux: W64.t;
+    
+    var mask:W64.t;
+    
+    leakages <- LeakAddr([]) :: leakages;
+    aux <- (W64.of_int 0);
+    mask <- aux;
+    leakages <- LeakAddr([]) :: leakages;
+    (aux_0, aux) <- adc_64 mask (W64.of_int 0) cf;
+    cf <- aux_0;
+    mask <- aux;
+    leakages <- LeakAddr([]) :: leakages;
+    aux <- (- mask);
+    mask <- aux;
+    return (mask);
+  }
+  
+  proc bN__addacc3 (a:W64.t Array3.t, b1:W64.t, b0:W64.t, k:int) : W64.t Array3.t = {
+    var aux: bool;
+    var aux_0: W64.t;
+    
+    var cf:bool;
+    
+    leakages <- LeakAddr([(k %% 3)]) :: leakages;
+    (aux, aux_0) <- adc_64 a.[(k %% 3)] b0 false;
+    cf <- aux;
+    leakages <- LeakAddr([(k %% 3)]) :: leakages;
+    a.[(k %% 3)] <- aux_0;
+    leakages <- LeakAddr([((k + 1) %% 3)]) :: leakages;
+    (aux, aux_0) <- adc_64 a.[((k + 1) %% 3)] b1 cf;
+    cf <- aux;
+    leakages <- LeakAddr([((k + 1) %% 3)]) :: leakages;
+    a.[((k + 1) %% 3)] <- aux_0;
+    leakages <- LeakAddr([((k + 2) %% 3)]) :: leakages;
+    (aux, aux_0) <- adc_64 a.[((k + 2) %% 3)] (W64.of_int 0) cf;
+    cf <- aux;
+    leakages <- LeakAddr([((k + 2) %% 3)]) :: leakages;
+    a.[((k + 2) %% 3)] <- aux_0;
+    return (a);
+  }
+  
+  proc bN__addacc3x2 (a:W64.t Array3.t, x:W64.t, y:W64.t, k:int) : W64.t Array3.t = {
+    var aux_5: bool;
+    var aux_4: bool;
+    var aux_3: bool;
+    var aux_2: bool;
+    var aux_1: bool;
+    var aux_0: W64.t;
+    var aux: W64.t;
+    
+    var b1:W64.t;
+    var b0:W64.t;
+    var t:W64.t;
+    var cf:bool;
+    var b2:W64.t;
+    var  _0:bool;
+    var  _1:bool;
+    var  _2:bool;
+    var  _3:bool;
+    
+    leakages <- LeakAddr([]) :: leakages;
+    (aux_0, aux) <- mulu_64 x y;
+    b1 <- aux_0;
+    b0 <- aux;
+    leakages <- LeakAddr([]) :: leakages;
+    aux_0 <- b0;
+    t <- aux_0;
+    leakages <- LeakAddr([]) :: leakages;
+    aux_0 <- (b0 `<<` (W8.of_int 1));
+    b0 <- aux_0;
+    leakages <- LeakAddr([]) :: leakages;
+    (aux_5, aux_4, aux_3, aux_2, aux_1, aux_0) <- SHLD_64 b1 t (W8.of_int 1);
+     _0 <- aux_5;
+    cf <- aux_4;
+     _1 <- aux_3;
+     _2 <- aux_2;
+     _3 <- aux_1;
+    b1 <- aux_0;
+    leakages <- LeakAddr([]) :: leakages;
+    aux_0 <- MOV_64 (W64.of_int 0);
+    b2 <- aux_0;
+    leakages <- LeakAddr([]) :: leakages;
+    (aux_5, aux_0) <- adc_64 b2 b2 cf;
+    cf <- aux_5;
+    b2 <- aux_0;
+    leakages <- LeakAddr([(k %% 3)]) :: leakages;
+    (aux_5, aux_0) <- adc_64 a.[(k %% 3)] b0 false;
+    cf <- aux_5;
+    leakages <- LeakAddr([(k %% 3)]) :: leakages;
+    a.[(k %% 3)] <- aux_0;
+    leakages <- LeakAddr([((k + 1) %% 3)]) :: leakages;
+    (aux_5, aux_0) <- adc_64 a.[((k + 1) %% 3)] b1 cf;
+    cf <- aux_5;
+    leakages <- LeakAddr([((k + 1) %% 3)]) :: leakages;
+    a.[((k + 1) %% 3)] <- aux_0;
+    leakages <- LeakAddr([((k + 2) %% 3)]) :: leakages;
+    (aux_5, aux_0) <- adc_64 a.[((k + 2) %% 3)] b2 cf;
+    cf <- aux_5;
+    leakages <- LeakAddr([((k + 2) %% 3)]) :: leakages;
+    a.[((k + 2) %% 3)] <- aux_0;
+    return (a);
+  }
+  
+  proc bN__load (a:W64.t Array11.t, ap:W64.t) : W64.t Array11.t = {
+    var aux: int;
+    var aux_0: W64.t;
+    
+    var i:int;
+    var t:W64.t;
+    
+    leakages <- LeakFor(0,11) :: LeakAddr([]) :: leakages;
+    i <- 0;
+    while (i < 11) {
+      leakages <- LeakAddr([(W64.to_uint (ap + (W64.of_int (8 * i))))]) :: leakages;
+      aux_0 <- (loadW64 Glob.mem (W64.to_uint (ap + (W64.of_int (8 * i)))));
+      t <- aux_0;
+      leakages <- LeakAddr([]) :: leakages;
+      aux_0 <- t;
+      leakages <- LeakAddr([i]) :: leakages;
+      a.[i] <- aux_0;
+      i <- i + 1;
+    }
+    return (a);
+  }
+  
+  proc bN_load (a:W64.t Array11.t, ap:W64.t) : W64.t Array11.t = {
+    var aux: W64.t Array11.t;
+    
+    
+    
+    leakages <- LeakAddr([]) :: leakages;
+    aux <@ bN__load (a, ap);
+    a <- aux;
+    return (a);
+  }
+  
+  proc bN_load_ (a:W64.t Array11.t, ap:W64.t) : W64.t Array11.t = {
+    var aux_0: W64.t;
+    var aux: W64.t Array11.t;
+    
+    
+    
+    leakages <- LeakAddr([]) :: leakages;
+    aux <- a;
+    a <- aux;
+    leakages <- LeakAddr([]) :: leakages;
+    aux_0 <- ap;
+    ap <- aux_0;
+    leakages <- LeakAddr([]) :: leakages;
+    aux <@ bN_load (a, ap);
+    a <- aux;
+    leakages <- LeakAddr([]) :: leakages;
+    aux <- a;
+    a <- aux;
+    return (a);
+  }
+  
+  proc bN__store (ap:W64.t, a:W64.t Array11.t) : unit = {
+    var aux: int;
+    var aux_0: W64.t;
+    
+    var i:int;
+    var t:W64.t;
+    
+    leakages <- LeakFor(0,11) :: LeakAddr([]) :: leakages;
+    i <- 0;
+    while (i < 11) {
+      leakages <- LeakAddr([i]) :: leakages;
+      aux_0 <- a.[i];
+      t <- aux_0;
+      leakages <- LeakAddr([]) :: leakages;
+      aux_0 <- t;
+      leakages <- LeakAddr([(W64.to_uint (ap + (W64.of_int (8 * i))))]) :: leakages;
+      Glob.mem <-
+      storeW64 Glob.mem (W64.to_uint (ap + (W64.of_int (8 * i)))) (aux_0);
+      i <- i + 1;
+    }
+    return ();
+  }
+  
+  proc bN_store_ (ap:W64.t, a:W64.t Array11.t) : unit = {
+    var aux: W64.t;
+    var aux_0: W64.t Array11.t;
+    
+    
+    
+    leakages <- LeakAddr([]) :: leakages;
+    aux <- ap;
+    ap <- aux;
+    leakages <- LeakAddr([]) :: leakages;
+    aux_0 <- a;
+    a <- aux_0;
+    leakages <- LeakAddr([]) :: leakages;
+    bN__store (ap, a);
+    return ();
+  }
+  
+  proc bN__eq_zf (a:W64.t Array11.t, b:W64.t Array11.t) : bool = {
+    var aux_5: bool;
+    var aux_4: bool;
+    var aux_3: bool;
+    var aux_2: bool;
+    var aux_1: bool;
+    var aux_0: int;
+    var aux: W64.t;
+    
+    var zf:bool;
+    var acc:W64.t;
+    var i:int;
+    var t:W64.t;
+    var  _0:bool;
+    var  _1:bool;
+    var  _2:bool;
+    var  _3:bool;
+    var  _4:W64.t;
+    
+    leakages <- LeakAddr([]) :: leakages;
+    aux <- (W64.of_int 0);
+    acc <- aux;
+    leakages <- LeakFor(0,11) :: LeakAddr([]) :: leakages;
+    i <- 0;
+    while (i < 11) {
+      leakages <- LeakAddr([i]) :: leakages;
+      aux <- a.[i];
+      t <- aux;
+      leakages <- LeakAddr([i]) :: leakages;
+      aux <- (t `^` b.[i]);
+      t <- aux;
+      leakages <- LeakAddr([]) :: leakages;
+      aux <- (acc `|` t);
+      acc <- aux;
+      i <- i + 1;
+    }
+    leakages <- LeakAddr([]) :: leakages;
+    (aux_5, aux_4, aux_3, aux_2, aux_1, aux) <- AND_64 acc acc;
+     _0 <- aux_5;
+     _1 <- aux_4;
+     _2 <- aux_3;
+     _3 <- aux_2;
+    zf <- aux_1;
+     _4 <- aux;
+    return (zf);
+  }
+  
+  proc bN_eq_zf (a:W64.t Array11.t, b:W64.t Array11.t) : bool = {
+    var aux: bool;
+    
+    var zf:bool;
+    
+    leakages <- LeakAddr([]) :: leakages;
+    aux <@ bN__eq_zf (a, b);
+    zf <- aux;
+    return (zf);
+  }
+  
+  proc bN_eq_zf_ (a:W64.t Array11.t, b:W64.t Array11.t) : bool = {
+    var aux_0: bool;
+    var aux: W64.t Array11.t;
+    
+    var zf:bool;
+    
+    leakages <- LeakAddr([]) :: leakages;
+    aux <- a;
+    a <- aux;
+    leakages <- LeakAddr([]) :: leakages;
+    aux <- b;
+    b <- aux;
+    leakages <- LeakAddr([]) :: leakages;
+    aux_0 <@ bN_eq_zf (a, b);
+    zf <- aux_0;
+    return (zf);
+  }
+  
+  proc bN_eq_ (a:W64.t Array11.t, b:W64.t Array11.t) : W64.t = {
+    var aux: bool;
+    var aux_0: W64.t;
+    
+    var res_0:W64.t;
+    var zf:bool;
+    var are_equal:W64.t;
+    
+    leakages <- LeakAddr([]) :: leakages;
+    aux <@ bN_eq_zf_ (a, b);
+    zf <- aux;
+    leakages <- LeakAddr([]) :: leakages;
+    aux_0 <- (W64.of_int 0);
+    res_0 <- aux_0;
+    leakages <- LeakAddr([]) :: leakages;
+    aux_0 <- (W64.of_int 1);
+    are_equal <- aux_0;
+    leakages <- LeakAddr([]) :: leakages;
+    aux_0 <- (zf ? are_equal : res_0);
+    res_0 <- aux_0;
+    return (res_0);
+  }
+  
+  proc bN__mov (r:W64.t Array11.t, a:W64.t Array11.t) : W64.t Array11.t = {
+    var aux: int;
+    var aux_0: W64.t;
+    
+    var i:int;
+    var t:W64.t;
+    
+    leakages <- LeakFor(0,11) :: LeakAddr([]) :: leakages;
+    i <- 0;
+    while (i < 11) {
+      leakages <- LeakAddr([i]) :: leakages;
+      aux_0 <- a.[i];
+      t <- aux_0;
+      leakages <- LeakAddr([]) :: leakages;
+      aux_0 <- t;
+      leakages <- LeakAddr([i]) :: leakages;
+      r.[i] <- aux_0;
+      i <- i + 1;
+    }
+    return (r);
+  }
+  
+  proc bN_mov (r:W64.t Array11.t, a:W64.t Array11.t) : W64.t Array11.t = {
+    var aux: W64.t Array11.t;
+    
+    
+    
+    leakages <- LeakAddr([]) :: leakages;
+    aux <@ bN__mov (r, a);
+    r <- aux;
+    return (r);
+  }
+  
+  proc bN_mov_ (r:W64.t Array11.t, a:W64.t Array11.t) : W64.t Array11.t = {
+    var aux: W64.t Array11.t;
+    
+    
+    
+    leakages <- LeakAddr([]) :: leakages;
+    aux <- r;
+    r <- aux;
+    leakages <- LeakAddr([]) :: leakages;
+    aux <- a;
+    a <- aux;
+    leakages <- LeakAddr([]) :: leakages;
+    aux <@ bN_mov (r, a);
+    r <- aux;
+    leakages <- LeakAddr([]) :: leakages;
+    aux <- r;
+    r <- aux;
+    return (r);
+  }
+  
+  proc bN__cmov (a:W64.t Array11.t, cond:bool, b:W64.t Array11.t) : W64.t Array11.t = {
+    var aux: int;
+    var aux_0: W64.t;
+    
+    var i:int;
+    var t:W64.t;
+    
+    leakages <- LeakFor(0,11) :: LeakAddr([]) :: leakages;
+    i <- 0;
+    while (i < 11) {
+      leakages <- LeakAddr([i]) :: leakages;
+      aux_0 <- a.[i];
+      t <- aux_0;
+      leakages <- LeakAddr([i]) :: leakages;
+      aux_0 <- (cond ? b.[i] : t);
+      t <- aux_0;
+      leakages <- LeakAddr([]) :: leakages;
+      aux_0 <- t;
+      leakages <- LeakAddr([i]) :: leakages;
+      a.[i] <- aux_0;
+      i <- i + 1;
+    }
+    return (a);
+  }
+  
+  proc bN_cmov (a:W64.t Array11.t, cond:bool, b:W64.t Array11.t) : W64.t Array11.t = {
+    var aux: W64.t Array11.t;
+    
+    
+    
+    leakages <- LeakAddr([]) :: leakages;
+    aux <@ bN__cmov (a, cond, b);
+    a <- aux;
+    return (a);
+  }
+  
+  proc bN_cmov_ (a:W64.t Array11.t, cond:bool, b:W64.t Array11.t) : W64.t Array11.t = {
+    var aux: W64.t Array11.t;
+    
+    
+    
+    leakages <- LeakAddr([]) :: leakages;
+    aux <- a;
+    a <- aux;
+    leakages <- LeakAddr([]) :: leakages;
+    aux <- b;
+    b <- aux;
+    leakages <- LeakAddr([]) :: leakages;
+    aux <@ bN_cmov (a, cond, b);
+    a <- aux;
+    leakages <- LeakAddr([]) :: leakages;
+    aux <- a;
+    a <- aux;
+    return (a);
+  }
+  
+  proc bN__cswap_mask (x:W64.t Array11.t, y:W64.t Array11.t, mask:W64.t) : 
+  W64.t Array11.t * W64.t Array11.t = {
+    var aux: int;
+    var aux_0: W64.t;
+    
+    var i:int;
+    var tmp1:W64.t;
+    
+    leakages <- LeakFor(0,11) :: LeakAddr([]) :: leakages;
+    i <- 0;
+    while (i < 11) {
+      leakages <- LeakAddr([i]) :: leakages;
+      aux_0 <- x.[i];
+      tmp1 <- aux_0;
+      leakages <- LeakAddr([i]) :: leakages;
+      aux_0 <- (tmp1 `^` y.[i]);
+      tmp1 <- aux_0;
+      leakages <- LeakAddr([]) :: leakages;
+      aux_0 <- (tmp1 `&` mask);
+      tmp1 <- aux_0;
+      leakages <- LeakAddr([i]) :: leakages;
+      aux_0 <- (x.[i] `^` tmp1);
+      leakages <- LeakAddr([i]) :: leakages;
+      x.[i] <- aux_0;
+      leakages <- LeakAddr([i]) :: leakages;
+      aux_0 <- (y.[i] `^` tmp1);
+      leakages <- LeakAddr([i]) :: leakages;
+      y.[i] <- aux_0;
+      i <- i + 1;
+    }
+    return (x, y);
+  }
+  
+  proc bN_cswap_mask (x:W64.t Array11.t, y:W64.t Array11.t, mask:W64.t) : 
+  W64.t Array11.t * W64.t Array11.t = {
+    var aux_0: W64.t Array11.t;
+    var aux: W64.t Array11.t;
+    
+    
+    
+    leakages <- LeakAddr([]) :: leakages;
+    (aux_0, aux) <@ bN__cswap_mask (x, y, mask);
+    x <- aux_0;
+    y <- aux;
+    return (x, y);
+  }
+  
+  proc bN_cswap_mask_ (x:W64.t Array11.t, y:W64.t Array11.t, mask:W64.t) : 
+  W64.t Array11.t * W64.t Array11.t = {
+    var aux_0: W64.t Array11.t;
+    var aux: W64.t Array11.t;
+    
+    
+    
+    leakages <- LeakAddr([]) :: leakages;
+    aux_0 <- x;
+    x <- aux_0;
+    leakages <- LeakAddr([]) :: leakages;
+    aux_0 <- y;
+    y <- aux_0;
+    leakages <- LeakAddr([]) :: leakages;
+    (aux_0, aux) <@ bN_cswap_mask (x, y, mask);
+    x <- aux_0;
+    y <- aux;
+    leakages <- LeakAddr([]) :: leakages;
+    aux_0 <- x;
+    x <- aux_0;
+    leakages <- LeakAddr([]) :: leakages;
+    aux_0 <- y;
+    y <- aux_0;
+    return (x, y);
+  }
+  
+  proc bN__fill (a:W64.t Array11.t, x:W64.t) : W64.t Array11.t = {
+    var aux: int;
+    var aux_0: W64.t;
+    
+    var i:int;
+    
+    leakages <- LeakFor(0,11) :: LeakAddr([]) :: leakages;
+    i <- 0;
+    while (i < 11) {
+      leakages <- LeakAddr([]) :: leakages;
+      aux_0 <- x;
+      leakages <- LeakAddr([i]) :: leakages;
+      a.[i] <- aux_0;
+      i <- i + 1;
+    }
+    return (a);
+  }
+  
+  proc bN_fill_ (a:W64.t Array11.t, x:W64.t) : W64.t Array11.t = {
+    var aux_0: W64.t;
+    var aux: W64.t Array11.t;
+    
+    
+    
+    leakages <- LeakAddr([]) :: leakages;
+    aux <- a;
+    a <- aux;
+    leakages <- LeakAddr([]) :: leakages;
+    aux_0 <- x;
+    x <- aux_0;
+    leakages <- LeakAddr([]) :: leakages;
+    aux <@ bN__fill (a, x);
+    a <- aux;
+    leakages <- LeakAddr([]) :: leakages;
+    aux <- a;
+    a <- aux;
+    return (a);
+  }
+  
+  proc bN_set0_ (a:W64.t Array11.t) : W64.t Array11.t = {
+    var aux: W64.t;
+    var aux_0: W64.t Array11.t;
+    
+    var t:W64.t;
+    
+    leakages <- LeakAddr([]) :: leakages;
+    aux <- (W64.of_int 0);
+    t <- aux;
+    leakages <- LeakAddr([]) :: leakages;
+    aux_0 <@ bN_fill_ (a, t);
+    a <- aux_0;
+    return (a);
+  }
+  
+  proc bN__and_mask (a:W64.t Array11.t, mask:W64.t) : W64.t Array11.t = {
+    var aux: int;
+    var aux_0: W64.t;
+    
+    var i:int;
+    
+    leakages <- LeakFor(0,11) :: LeakAddr([]) :: leakages;
+    i <- 0;
+    while (i < 11) {
+      leakages <- LeakAddr([i]) :: leakages;
+      aux_0 <- (a.[i] `&` mask);
+      leakages <- LeakAddr([i]) :: leakages;
+      a.[i] <- aux_0;
+      i <- i + 1;
+    }
+    return (a);
+  }
+  
+  proc bN_and_mask (a:W64.t Array11.t, mask:W64.t) : W64.t Array11.t = {
+    var aux: W64.t Array11.t;
+    
+    
+    
+    leakages <- LeakAddr([]) :: leakages;
+    aux <@ bN__and_mask (a, mask);
+    a <- aux;
+    return (a);
+  }
+  
+  proc bN_and_mask_ (a:W64.t Array11.t, mask:W64.t) : W64.t Array11.t = {
+    var aux_0: W64.t;
+    var aux: W64.t Array11.t;
+    
+    
+    
+    leakages <- LeakAddr([]) :: leakages;
+    aux <- a;
+    a <- aux;
+    leakages <- LeakAddr([]) :: leakages;
+    aux_0 <- mask;
+    mask <- aux_0;
+    leakages <- LeakAddr([]) :: leakages;
+    aux <@ bN_and_mask (a, mask);
+    a <- aux;
+    leakages <- LeakAddr([]) :: leakages;
+    aux <- a;
+    a <- aux;
+    return (a);
+  }
+  
+  proc bN__addc1U (a:W64.t Array11.t, b:W64.t Array11.t, cf:bool) : bool *
+                                                                    W64.t Array11.t = {
+    var aux_1: bool;
+    var aux: int;
+    var aux_0: W64.t;
+    
+    var i:int;
+    var t:W64.t;
+    
+    leakages <- LeakFor(1,11) :: LeakAddr([]) :: leakages;
+    i <- 1;
+    while (i < 11) {
+      leakages <- LeakAddr([i]) :: leakages;
+      aux_0 <- b.[i];
+      t <- aux_0;
+      leakages <- LeakAddr([i]) :: leakages;
+      (aux_1, aux_0) <- adc_64 a.[i] t cf;
+      cf <- aux_1;
+      leakages <- LeakAddr([i]) :: leakages;
+      a.[i] <- aux_0;
+      i <- i + 1;
+    }
+    return (cf, a);
+  }
+  
+  proc bN_addc1U (a:W64.t Array11.t, b:W64.t Array11.t, cf:bool) : bool *
+                                                                   W64.t Array11.t = {
+    var aux: bool;
+    var aux_0: W64.t Array11.t;
+    
+    
+    
+    leakages <- LeakAddr([]) :: leakages;
+    (aux, aux_0) <@ bN__addc1U (a, b, cf);
+    cf <- aux;
+    a <- aux_0;
+    return (cf, a);
+  }
+  
+  proc bN_addc1U_ (a:W64.t Array11.t, b:W64.t Array11.t, cf:bool) : bool *
+                                                                    W64.t Array11.t = {
+    var aux_0: bool;
+    var aux: W64.t Array11.t;
+    
+    
+    
+    leakages <- LeakAddr([]) :: leakages;
+    aux <- a;
+    a <- aux;
+    leakages <- LeakAddr([]) :: leakages;
+    aux <- b;
+    b <- aux;
+    leakages <- LeakAddr([]) :: leakages;
+    (aux_0, aux) <@ bN_addc1U (a, b, cf);
+    cf <- aux_0;
+    a <- aux;
+    leakages <- LeakAddr([]) :: leakages;
+    aux <- a;
+    a <- aux;
+    return (cf, a);
+  }
+  
+  proc bN_addU_ (a:W64.t Array11.t, b:W64.t Array11.t) : bool *
+                                                         W64.t Array11.t = {
+    var aux_0: bool;
+    var aux: W64.t;
+    var aux_1: W64.t Array11.t;
+    
+    var cf:bool;
+    var t:W64.t;
+    
+    leakages <- LeakAddr([0]) :: leakages;
+    aux <- b.[0];
+    t <- aux;
+    leakages <- LeakAddr([0]) :: leakages;
+    (aux_0, aux) <- adc_64 a.[0] t false;
+    cf <- aux_0;
+    leakages <- LeakAddr([0]) :: leakages;
+    a.[0] <- aux;
+    leakages <- LeakAddr([]) :: leakages;
+    (aux_0, aux_1) <@ bN_addc1U_ (a, b, cf);
+    cf <- aux_0;
+    a <- aux_1;
+    return (cf, a);
+  }
+  
+  proc bN__addc1 (r:W64.t Array11.t, a:W64.t Array11.t, b:W64.t Array11.t,
+                  cf:bool) : bool * W64.t Array11.t = {
+    var aux_1: bool;
+    var aux: int;
+    var aux_0: W64.t;
+    
+    var i:int;
+    var t:W64.t;
+    
+    leakages <- LeakFor(1,11) :: LeakAddr([]) :: leakages;
+    i <- 1;
+    while (i < 11) {
+      leakages <- LeakAddr([i]) :: leakages;
+      aux_0 <- a.[i];
+      t <- aux_0;
+      leakages <- LeakAddr([i]) :: leakages;
+      (aux_1, aux_0) <- adc_64 t b.[i] cf;
+      cf <- aux_1;
+      t <- aux_0;
+      leakages <- LeakAddr([]) :: leakages;
+      aux_0 <- t;
+      leakages <- LeakAddr([i]) :: leakages;
+      r.[i] <- aux_0;
+      i <- i + 1;
+    }
+    return (cf, r);
+  }
+  
+  proc bN_addc1 (r:W64.t Array11.t, a:W64.t Array11.t, b:W64.t Array11.t,
+                 cf:bool) : bool * W64.t Array11.t = {
+    var aux: bool;
+    var aux_0: W64.t Array11.t;
+    
+    
+    
+    leakages <- LeakAddr([]) :: leakages;
+    (aux, aux_0) <@ bN__addc1 (r, a, b, cf);
+    cf <- aux;
+    r <- aux_0;
+    return (cf, r);
+  }
+  
+  proc bN_addc1_ (r:W64.t Array11.t, a:W64.t Array11.t, b:W64.t Array11.t,
+                  cf:bool) : bool * W64.t Array11.t = {
+    var aux_0: bool;
+    var aux: W64.t Array11.t;
+    
+    
+    
+    leakages <- LeakAddr([]) :: leakages;
+    aux <- r;
+    r <- aux;
+    leakages <- LeakAddr([]) :: leakages;
+    aux <- a;
+    a <- aux;
+    leakages <- LeakAddr([]) :: leakages;
+    aux <- b;
+    b <- aux;
+    leakages <- LeakAddr([]) :: leakages;
+    (aux_0, aux) <@ bN_addc1 (r, a, b, cf);
+    cf <- aux_0;
+    r <- aux;
+    leakages <- LeakAddr([]) :: leakages;
+    aux <- r;
+    r <- aux;
+    return (cf, r);
+  }
+  
+  proc bN_add_ (r:W64.t Array11.t, a:W64.t Array11.t, b:W64.t Array11.t) : 
+  bool * W64.t Array11.t = {
+    var aux_0: bool;
+    var aux: W64.t;
+    var aux_1: W64.t Array11.t;
+    
+    var cf:bool;
+    var t:W64.t;
+    
+    leakages <- LeakAddr([0]) :: leakages;
+    aux <- a.[0];
+    t <- aux;
+    leakages <- LeakAddr([0]) :: leakages;
+    (aux_0, aux) <- adc_64 t b.[0] false;
+    cf <- aux_0;
+    t <- aux;
+    leakages <- LeakAddr([]) :: leakages;
+    aux <- t;
+    leakages <- LeakAddr([0]) :: leakages;
+    r.[0] <- aux;
+    leakages <- LeakAddr([]) :: leakages;
+    (aux_0, aux_1) <@ bN_addc1_ (r, a, b, cf);
+    cf <- aux_0;
+    r <- aux_1;
+    return (cf, a);
+  }
+  
+  proc bN__subc1U (a:W64.t Array11.t, b:W64.t Array11.t, cf:bool) : bool *
+                                                                    W64.t Array11.t = {
+    var aux_1: bool;
+    var aux: int;
+    var aux_0: W64.t;
+    
+    var i:int;
+    var t:W64.t;
+    
+    leakages <- LeakFor(1,11) :: LeakAddr([]) :: leakages;
+    i <- 1;
+    while (i < 11) {
+      leakages <- LeakAddr([i]) :: leakages;
+      aux_0 <- b.[i];
+      t <- aux_0;
+      leakages <- LeakAddr([i]) :: leakages;
+      (aux_1, aux_0) <- sbb_64 a.[i] t cf;
+      cf <- aux_1;
+      leakages <- LeakAddr([i]) :: leakages;
+      a.[i] <- aux_0;
+      i <- i + 1;
+    }
+    return (cf, a);
+  }
+  
+  proc bN_subc1U (a:W64.t Array11.t, b:W64.t Array11.t, cf:bool) : bool *
+                                                                   W64.t Array11.t = {
+    var aux: bool;
+    var aux_0: W64.t Array11.t;
+    
+    
+    
+    leakages <- LeakAddr([]) :: leakages;
+    (aux, aux_0) <@ bN__subc1U (a, b, cf);
+    cf <- aux;
+    a <- aux_0;
+    return (cf, a);
+  }
+  
+  proc bN_subc1U_ (a:W64.t Array11.t, b:W64.t Array11.t, cf:bool) : bool *
+                                                                    W64.t Array11.t = {
+    var aux_0: bool;
+    var aux: W64.t Array11.t;
+    
+    
+    
+    leakages <- LeakAddr([]) :: leakages;
+    aux <- a;
+    a <- aux;
+    leakages <- LeakAddr([]) :: leakages;
+    aux <- b;
+    b <- aux;
+    leakages <- LeakAddr([]) :: leakages;
+    (aux_0, aux) <@ bN_subc1U (a, b, cf);
+    cf <- aux_0;
+    a <- aux;
+    leakages <- LeakAddr([]) :: leakages;
+    aux <- a;
+    a <- aux;
+    return (cf, a);
+  }
+  
+  proc bN_subU_ (a:W64.t Array11.t, b:W64.t Array11.t) : bool *
+                                                         W64.t Array11.t = {
+    var aux_0: bool;
+    var aux: W64.t;
+    var aux_1: W64.t Array11.t;
+    
+    var cf:bool;
+    var t:W64.t;
+    
+    leakages <- LeakAddr([0]) :: leakages;
+    aux <- b.[0];
+    t <- aux;
+    leakages <- LeakAddr([0]) :: leakages;
+    (aux_0, aux) <- sbb_64 a.[0] t false;
+    cf <- aux_0;
+    leakages <- LeakAddr([0]) :: leakages;
+    a.[0] <- aux;
+    leakages <- LeakAddr([]) :: leakages;
+    (aux_0, aux_1) <@ bN_subc1U_ (a, b, cf);
+    cf <- aux_0;
+    a <- aux_1;
+    return (cf, a);
+  }
+  
+  proc bN__subc1 (r:W64.t Array11.t, a:W64.t Array11.t, b:W64.t Array11.t,
+                  cf:bool) : bool * W64.t Array11.t = {
+    var aux_1: bool;
+    var aux: int;
+    var aux_0: W64.t;
+    
+    var i:int;
+    var t:W64.t;
+    
+    leakages <- LeakFor(1,11) :: LeakAddr([]) :: leakages;
+    i <- 1;
+    while (i < 11) {
+      leakages <- LeakAddr([i]) :: leakages;
+      aux_0 <- a.[i];
+      t <- aux_0;
+      leakages <- LeakAddr([i]) :: leakages;
+      (aux_1, aux_0) <- sbb_64 t b.[i] cf;
+      cf <- aux_1;
+      t <- aux_0;
+      leakages <- LeakAddr([]) :: leakages;
+      aux_0 <- t;
+      leakages <- LeakAddr([i]) :: leakages;
+      r.[i] <- aux_0;
+      i <- i + 1;
+    }
+    return (cf, r);
+  }
+  
+  proc bN_subc1 (r:W64.t Array11.t, a:W64.t Array11.t, b:W64.t Array11.t,
+                 cf:bool) : bool * W64.t Array11.t = {
+    var aux: bool;
+    var aux_0: W64.t Array11.t;
+    
+    
+    
+    leakages <- LeakAddr([]) :: leakages;
+    (aux, aux_0) <@ bN__subc1 (r, a, b, cf);
+    cf <- aux;
+    r <- aux_0;
+    return (cf, r);
+  }
+  
+  proc bN_subc1_ (r:W64.t Array11.t, a:W64.t Array11.t, b:W64.t Array11.t,
+                  cf:bool) : bool * W64.t Array11.t = {
+    var aux_0: bool;
+    var aux: W64.t Array11.t;
+    
+    
+    
+    leakages <- LeakAddr([]) :: leakages;
+    aux <- r;
+    r <- aux;
+    leakages <- LeakAddr([]) :: leakages;
+    aux <- a;
+    a <- aux;
+    leakages <- LeakAddr([]) :: leakages;
+    aux <- b;
+    b <- aux;
+    leakages <- LeakAddr([]) :: leakages;
+    (aux_0, aux) <@ bN_subc1 (r, a, b, cf);
+    cf <- aux_0;
+    r <- aux;
+    leakages <- LeakAddr([]) :: leakages;
+    aux <- r;
+    r <- aux;
+    return (cf, r);
+  }
+  
+  proc bN_sub_ (r:W64.t Array11.t, a:W64.t Array11.t, b:W64.t Array11.t) : 
+  bool * W64.t Array11.t = {
+    var aux_0: bool;
+    var aux: W64.t;
+    var aux_1: W64.t Array11.t;
+    
+    var cf:bool;
+    var t:W64.t;
+    
+    leakages <- LeakAddr([0]) :: leakages;
+    aux <- a.[0];
+    t <- aux;
+    leakages <- LeakAddr([0]) :: leakages;
+    (aux_0, aux) <- sbb_64 t b.[0] false;
+    cf <- aux_0;
+    t <- aux;
+    leakages <- LeakAddr([]) :: leakages;
+    aux <- t;
+    leakages <- LeakAddr([0]) :: leakages;
+    r.[0] <- aux;
+    leakages <- LeakAddr([]) :: leakages;
+    (aux_0, aux_1) <@ bN_subc1_ (r, a, b, cf);
+    cf <- aux_0;
+    r <- aux_1;
+    return (cf, r);
+  }
+  
+  proc bN__ltc1_cf (a:W64.t Array11.t, b:W64.t Array11.t, cf:bool) : 
+  bool = {
+    var aux_1: bool;
+    var aux: int;
+    var aux_0: W64.t;
+    
+    var i:int;
+    var t:W64.t;
+    
+    leakages <- LeakFor(1,11) :: LeakAddr([]) :: leakages;
+    i <- 1;
+    while (i < 11) {
+      leakages <- LeakAddr([i]) :: leakages;
+      aux_0 <- a.[i];
+      t <- aux_0;
+      leakages <- LeakAddr([i]) :: leakages;
+      (aux_1, aux_0) <- sbb_64 t b.[i] cf;
+      cf <- aux_1;
+      t <- aux_0;
+      i <- i + 1;
+    }
+    return (cf);
+  }
+  
+  proc bN_ltc1_cf (a:W64.t Array11.t, b:W64.t Array11.t, cf:bool) : bool = {
+    var aux: bool;
+    
+    
+    
+    leakages <- LeakAddr([]) :: leakages;
+    aux <@ bN__ltc1_cf (a, b, cf);
+    cf <- aux;
+    return (cf);
+  }
+  
+  proc bN_ltc1_cf_ (a:W64.t Array11.t, b:W64.t Array11.t, cf:bool) : 
+  bool = {
+    var aux_0: bool;
+    var aux: W64.t Array11.t;
+    
+    
+    
+    leakages <- LeakAddr([]) :: leakages;
+    aux <- a;
+    a <- aux;
+    leakages <- LeakAddr([]) :: leakages;
+    aux <- b;
+    b <- aux;
+    leakages <- LeakAddr([]) :: leakages;
+    aux_0 <@ bN_ltc1_cf (a, b, cf);
+    cf <- aux_0;
+    return (cf);
+  }
+  
+  proc bN_lt_cf_ (a:W64.t Array11.t, b:W64.t Array11.t) : bool = {
+    var aux_0: bool;
+    var aux: W64.t;
+    
+    var cf:bool;
+    var t:W64.t;
+    
+    leakages <- LeakAddr([0]) :: leakages;
+    aux <- a.[0];
+    t <- aux;
+    leakages <- LeakAddr([0]) :: leakages;
+    (aux_0, aux) <- sbb_64 t b.[0] false;
+    cf <- aux_0;
+    t <- aux;
+    leakages <- LeakAddr([]) :: leakages;
+    aux_0 <@ bN_ltc1_cf_ (a, b, cf);
+    cf <- aux_0;
+    return (cf);
+  }
+  
+  proc bN_caddU_ (x:W64.t Array11.t, cf:bool, y:W64.t Array11.t) : W64.t Array11.t = {
+    var aux_1: bool;
+    var aux_0: W64.t;
+    var aux: W64.t Array11.t;
+    
+    var _tmp:W64.t Array11.t;
+    var tmp:W64.t Array11.t;
+    var mask:W64.t;
+    var  _0:bool;
+    _tmp <- witness;
+    tmp <- witness;
+    leakages <- LeakAddr([]) :: leakages;
+    aux <- _tmp;
+    tmp <- aux;
+    leakages <- LeakAddr([]) :: leakages;
+    aux <@ bN_mov_ (tmp, y);
+    tmp <- aux;
+    leakages <- LeakAddr([]) :: leakages;
+    aux_0 <@ bN__cf_mask (cf);
+    mask <- aux_0;
+    leakages <- LeakAddr([]) :: leakages;
+    aux <@ bN_and_mask_ (tmp, mask);
+    tmp <- aux;
+    leakages <- LeakAddr([]) :: leakages;
+    (aux_1, aux) <@ bN_addU_ (x, tmp);
+     _0 <- aux_1;
+    x <- aux;
+    return (x);
+  }
+  
+  proc bN__muln_innerloop (x:W64.t Array3.t, k:int, istart:int, iend:int,
+                           a:W64.t Array11.t, b:W64.t Array11.t) : W64.t Array3.t = {
+    var aux: int;
+    var aux_1: W64.t;
+    var aux_0: W64.t;
+    var aux_2: W64.t Array3.t;
+    
+    var i:int;
+    var j:int;
+    var t0:W64.t;
+    var t1:W64.t;
+    
+    leakages <- LeakFor(istart,iend) :: LeakAddr([]) :: leakages;
+    aux <- iend;
+    i <- istart;
+    while (i < aux) {
+      leakages <- LeakAddr([]) :: leakages;
+      aux <- (k - i);
+      j <- aux;
+      leakages <- LeakAddr([i]) :: leakages;
+      aux_1 <- a.[i];
+      t0 <- aux_1;
+      leakages <- LeakAddr([j]) :: leakages;
+      (aux_1, aux_0) <- mulu_64 t0 b.[j];
+      t1 <- aux_1;
+      t0 <- aux_0;
+      leakages <- LeakAddr([]) :: leakages;
+      aux_2 <@ bN__addacc3 (x, t1, t0, k);
+      x <- aux_2;
+      i <- i + 1;
+    }
+    return (x);
+  }
+  
+  proc bN__muln (r:W64.t Array22.t, a:W64.t Array11.t, b:W64.t Array11.t) : 
+  W64.t Array22.t = {
+    var aux_1: int;
+    var aux_0: W64.t;
+    var aux: W64.t;
+    var aux_2: W64.t Array3.t;
+    
+    var t0:W64.t;
+    var t1:W64.t;
+    var x:W64.t Array3.t;
+    var k:int;
+    x <- witness;
+    leakages <- LeakAddr([0]) :: leakages;
+    aux_0 <- a.[0];
+    t0 <- aux_0;
+    leakages <- LeakAddr([0]) :: leakages;
+    (aux_0, aux) <- mulu_64 t0 b.[0];
+    t1 <- aux_0;
+    t0 <- aux;
+    leakages <- LeakAddr([]) :: leakages;
+    aux_0 <- t0;
+    leakages <- LeakAddr([0]) :: leakages;
+    r.[0] <- aux_0;
+    leakages <- LeakAddr([]) :: leakages;
+    aux_0 <- t1;
+    leakages <- LeakAddr([1]) :: leakages;
+    x.[1] <- aux_0;
+    leakages <- LeakAddr([]) :: leakages;
+    aux_0 <- (W64.of_int 0);
+    leakages <- LeakAddr([2]) :: leakages;
+    x.[2] <- aux_0;
+    leakages <- LeakAddr([]) :: leakages;
+    aux_0 <- (W64.of_int 0);
+    leakages <- LeakAddr([0]) :: leakages;
+    x.[0] <- aux_0;
+    leakages <- LeakFor(1,11) :: LeakAddr([]) :: leakages;
+    k <- 1;
+    while (k < 11) {
+      leakages <- LeakAddr([]) :: leakages;
+      aux_2 <@ bN__muln_innerloop (x, k, 0, (k + 1), a, b);
+      x <- aux_2;
+      leakages <- LeakAddr([(k %% 3)]) :: leakages;
+      aux_0 <- x.[(k %% 3)];
+      t0 <- aux_0;
+      leakages <- LeakAddr([]) :: leakages;
+      aux_0 <- (W64.of_int 0);
+      leakages <- LeakAddr([(k %% 3)]) :: leakages;
+      x.[(k %% 3)] <- aux_0;
+      leakages <- LeakAddr([]) :: leakages;
+      aux_0 <- t0;
+      leakages <- LeakAddr([k]) :: leakages;
+      r.[k] <- aux_0;
+      k <- k + 1;
+    }
+    leakages <- LeakFor(11,((2 * 11) - 1)) :: LeakAddr([]) :: leakages;
+    aux_1 <- ((2 * 11) - 1);
+    k <- 11;
+    while (k < aux_1) {
+      leakages <- LeakAddr([]) :: leakages;
+      aux_2 <@ bN__muln_innerloop (x, k, ((k - 11) + 1), 11, a, b);
+      x <- aux_2;
+      leakages <- LeakAddr([(k %% 3)]) :: leakages;
+      aux_0 <- x.[(k %% 3)];
+      t0 <- aux_0;
+      leakages <- LeakAddr([]) :: leakages;
+      aux_0 <- (W64.of_int 0);
+      leakages <- LeakAddr([(k %% 3)]) :: leakages;
+      x.[(k %% 3)] <- aux_0;
+      leakages <- LeakAddr([]) :: leakages;
+      aux_0 <- t0;
+      leakages <- LeakAddr([k]) :: leakages;
+      r.[k] <- aux_0;
+      k <- k + 1;
+    }
+    leakages <- LeakAddr([(((2 * 11) - 1) %% 3)]) :: leakages;
+    aux_0 <- x.[(((2 * 11) - 1) %% 3)];
+    leakages <- LeakAddr([((2 * 11) - 1)]) :: leakages;
+    r.[((2 * 11) - 1)] <- aux_0;
+    return (r);
+  }
+  
+  proc bN_muln (r:W64.t Array22.t, a:W64.t Array11.t, b:W64.t Array11.t) : 
+  W64.t Array22.t = {
+    var aux: W64.t Array22.t;
+    
+    
+    
+    leakages <- LeakAddr([]) :: leakages;
+    aux <@ bN__muln (r, a, b);
+    r <- aux;
+    return (r);
+  }
+  
+  proc bN_muln_ (r:W64.t Array22.t, a:W64.t Array11.t, b:W64.t Array11.t) : 
+  W64.t Array22.t = {
+    var aux_0: W64.t Array11.t;
+    var aux: W64.t Array22.t;
+    
+    
+    
+    leakages <- LeakAddr([]) :: leakages;
+    aux <- r;
+    r <- aux;
+    leakages <- LeakAddr([]) :: leakages;
+    aux_0 <- a;
+    a <- aux_0;
+    leakages <- LeakAddr([]) :: leakages;
+    aux_0 <- b;
+    b <- aux_0;
+    leakages <- LeakAddr([]) :: leakages;
+    aux <@ bN_muln (r, a, b);
+    r <- aux;
+    leakages <- LeakAddr([]) :: leakages;
+    aux <- r;
+    r <- aux;
+    return (r);
+  }
+  
+  proc bN__sqrn_innerloop (x:W64.t Array3.t, k:int, istart:int, iend:int,
+                           a:W64.t Array11.t) : W64.t Array3.t = {
+    var aux: int;
+    var aux_0: W64.t;
+    var aux_1: W64.t Array3.t;
+    
+    var i:int;
+    var j:int;
+    var ti:W64.t;
+    var tj:W64.t;
+    
+    leakages <- LeakFor(istart,iend) :: LeakAddr([]) :: leakages;
+    aux <- iend;
+    i <- istart;
+    while (i < aux) {
+      leakages <- LeakAddr([]) :: leakages;
+      aux <- (k - i);
+      j <- aux;
+      leakages <- LeakAddr([i]) :: leakages;
+      aux_0 <- a.[i];
+      ti <- aux_0;
+      leakages <- LeakAddr([j]) :: leakages;
+      aux_0 <- a.[j];
+      tj <- aux_0;
+      leakages <- LeakAddr([]) :: leakages;
+      aux_1 <@ bN__addacc3x2 (x, ti, tj, k);
+      x <- aux_1;
+      i <- i + 1;
+    }
+    return (x);
+  }
+  
+  proc bN__sqrn (r:W64.t Array22.t, a:W64.t Array11.t) : W64.t Array22.t = {
+    var aux_1: int;
+    var aux_0: W64.t;
+    var aux: W64.t;
+    var aux_2: W64.t Array3.t;
+    
+    var t0:W64.t;
+    var t1:W64.t;
+    var x:W64.t Array3.t;
+    var k:int;
+    x <- witness;
+    leakages <- LeakAddr([0]) :: leakages;
+    aux_0 <- a.[0];
+    t0 <- aux_0;
+    leakages <- LeakAddr([]) :: leakages;
+    (aux_0, aux) <- mulu_64 t0 t0;
+    t1 <- aux_0;
+    t0 <- aux;
+    leakages <- LeakAddr([]) :: leakages;
+    aux_0 <- t0;
+    leakages <- LeakAddr([0]) :: leakages;
+    r.[0] <- aux_0;
+    leakages <- LeakAddr([]) :: leakages;
+    aux_0 <- t1;
+    leakages <- LeakAddr([1]) :: leakages;
+    x.[1] <- aux_0;
+    leakages <- LeakAddr([]) :: leakages;
+    aux_0 <- (W64.of_int 0);
+    leakages <- LeakAddr([2]) :: leakages;
+    x.[2] <- aux_0;
+    leakages <- LeakAddr([]) :: leakages;
+    aux_0 <- (W64.of_int 0);
+    leakages <- LeakAddr([0]) :: leakages;
+    x.[0] <- aux_0;
+    leakages <- LeakFor(1,11) :: LeakAddr([]) :: leakages;
+    k <- 1;
+    while (k < 11) {
+      leakages <- LeakAddr([]) :: leakages;
+      aux_2 <@ bN__sqrn_innerloop (x, k, 0, ((k + 1) %/ 2), a);
+      x <- aux_2;
+      leakages <- LeakCond(((k %% 2) = 0)) :: LeakAddr([]) :: leakages;
+      if (((k %% 2) = 0)) {
+        leakages <- LeakAddr([(k %/ 2)]) :: leakages;
+        aux_0 <- a.[(k %/ 2)];
+        t0 <- aux_0;
+        leakages <- LeakAddr([]) :: leakages;
+        (aux_0, aux) <- mulu_64 t0 t0;
+        t1 <- aux_0;
+        t0 <- aux;
+        leakages <- LeakAddr([]) :: leakages;
+        aux_2 <@ bN__addacc3 (x, t1, t0, k);
+        x <- aux_2;
+      } else {
+        
+      }
+      leakages <- LeakAddr([(k %% 3)]) :: leakages;
+      aux_0 <- x.[(k %% 3)];
+      t0 <- aux_0;
+      leakages <- LeakAddr([]) :: leakages;
+      aux_0 <- (W64.of_int 0);
+      leakages <- LeakAddr([(k %% 3)]) :: leakages;
+      x.[(k %% 3)] <- aux_0;
+      leakages <- LeakAddr([]) :: leakages;
+      aux_0 <- t0;
+      leakages <- LeakAddr([k]) :: leakages;
+      r.[k] <- aux_0;
+      k <- k + 1;
+    }
+    leakages <- LeakFor(11,((2 * 11) - 1)) :: LeakAddr([]) :: leakages;
+    aux_1 <- ((2 * 11) - 1);
+    k <- 11;
+    while (k < aux_1) {
+      leakages <- LeakAddr([]) :: leakages;
+      aux_2 <@ bN__sqrn_innerloop (x, k, ((k - 11) + 1), ((k + 1) %/ 2), a);
+      x <- aux_2;
+      leakages <- LeakCond(((k %% 2) = 0)) :: LeakAddr([]) :: leakages;
+      if (((k %% 2) = 0)) {
+        leakages <- LeakAddr([(k %/ 2)]) :: leakages;
+        aux_0 <- a.[(k %/ 2)];
+        t0 <- aux_0;
+        leakages <- LeakAddr([]) :: leakages;
+        (aux_0, aux) <- mulu_64 t0 t0;
+        t1 <- aux_0;
+        t0 <- aux;
+        leakages <- LeakAddr([]) :: leakages;
+        aux_2 <@ bN__addacc3 (x, t1, t0, k);
+        x <- aux_2;
+      } else {
+        
+      }
+      leakages <- LeakAddr([(k %% 3)]) :: leakages;
+      aux_0 <- x.[(k %% 3)];
+      t0 <- aux_0;
+      leakages <- LeakAddr([]) :: leakages;
+      aux_0 <- (W64.of_int 0);
+      leakages <- LeakAddr([(k %% 3)]) :: leakages;
+      x.[(k %% 3)] <- aux_0;
+      leakages <- LeakAddr([]) :: leakages;
+      aux_0 <- t0;
+      leakages <- LeakAddr([k]) :: leakages;
+      r.[k] <- aux_0;
+      k <- k + 1;
+    }
+    leakages <- LeakAddr([(((2 * 11) - 1) %% 3)]) :: leakages;
+    aux_0 <- x.[(((2 * 11) - 1) %% 3)];
+    leakages <- LeakAddr([((2 * 11) - 1)]) :: leakages;
+    r.[((2 * 11) - 1)] <- aux_0;
+    return (r);
+  }
+  
+  proc bN_sqrn (r:W64.t Array22.t, a:W64.t Array11.t) : W64.t Array22.t = {
+    var aux: W64.t Array22.t;
+    
+    
+    
+    leakages <- LeakAddr([]) :: leakages;
+    aux <@ bN__sqrn (r, a);
+    r <- aux;
+    return (r);
+  }
+  
+  proc bN_sqrn_ (r:W64.t Array22.t, a:W64.t Array11.t) : W64.t Array22.t = {
+    var aux_0: W64.t Array11.t;
+    var aux: W64.t Array22.t;
+    
+    
+    
+    leakages <- LeakAddr([]) :: leakages;
+    aux <- r;
+    r <- aux;
+    leakages <- LeakAddr([]) :: leakages;
+    aux_0 <- a;
+    a <- aux_0;
+    leakages <- LeakAddr([]) :: leakages;
+    aux <@ bN_sqrn (r, a);
+    r <- aux;
+    leakages <- LeakAddr([]) :: leakages;
+    aux <- r;
+    r <- aux;
+    return (r);
+  }
+  
+  proc bN_cminusP_ (x:W64.t Array11.t, mP:W64.t Array11.t, lastbit:W64.t) : 
+  W64.t Array11.t = {
+    var aux_5: bool;
+    var aux_4: bool;
+    var aux_3: bool;
+    var aux_2: bool;
+    var aux_0: bool;
+    var aux_1: W64.t;
+    var aux: W64.t Array11.t;
+    
+    var _tmp:W64.t Array11.t;
+    var tmp:W64.t Array11.t;
+    var _cf:bool;
+    var  _0:bool;
+    var  _1:bool;
+    var  _2:bool;
+    var  _3:bool;
+    var  _4:bool;
+    var  _5:W64.t;
+    _tmp <- witness;
+    tmp <- witness;
+    leakages <- LeakAddr([]) :: leakages;
+    aux <- _tmp;
+    tmp <- aux;
+    leakages <- LeakAddr([]) :: leakages;
+    aux <@ bN_mov_ (tmp, x);
+    tmp <- aux;
+    leakages <- LeakAddr([]) :: leakages;
+    (aux_5, aux) <@ bN_addU_ (tmp, mP);
+    _cf <- aux_5;
+    tmp <- aux;
+    leakages <- LeakAddr([]) :: leakages;
+    (aux_5, aux_1) <- adc_64 lastbit (W64.of_int 0) _cf;
+     _0 <- aux_5;
+    lastbit <- aux_1;
+    leakages <- LeakAddr([]) :: leakages;
+    (aux_5, aux_4, aux_3, aux_2, aux_0, aux_1) <- NEG_64 lastbit;
+     _1 <- aux_5;
+    _cf <- aux_4;
+     _2 <- aux_3;
+     _3 <- aux_2;
+     _4 <- aux_0;
+     _5 <- aux_1;
+    leakages <- LeakAddr([]) :: leakages;
+    aux <@ bN_cmov_ (x, _cf, tmp);
+    x <- aux;
+    return (x);
+  }
+  
+  proc bN__mont_redM (r:W64.t Array11.t, a:W64.t Array22.t,
+                      _P:W64.t Array11.t, _mP:W64.t Array11.t, _U0:W64.t) : 
+  W64.t Array11.t = {
+    var aux_4: bool;
+    var aux_0: int;
+    var aux_3: W64.t;
+    var aux: W64.t;
+    var aux_2: W64.t Array3.t;
+    var aux_1: W64.t Array11.t;
+    
+    var x:W64.t Array3.t;
+    var p:W64.t Array11.t;
+    var k:int;
+    var zero:W64.t;
+    var t0:W64.t;
+    var t1:W64.t;
+    var lastbit:W64.t;
+    var cf:bool;
+    var mP:W64.t Array11.t;
+    var  _0:W64.t;
+    var  _1:bool;
+    p <- witness;
+    mP <- witness;
+    x <- witness;
+    leakages <- LeakAddr([]) :: leakages;
+    aux_3 <- (W64.of_int 0);
+    leakages <- LeakAddr([0]) :: leakages;
+    x.[0] <- aux_3;
+    leakages <- LeakAddr([]) :: leakages;
+    aux_3 <- (W64.of_int 0);
+    leakages <- LeakAddr([1]) :: leakages;
+    x.[1] <- aux_3;
+    leakages <- LeakAddr([]) :: leakages;
+    aux_3 <- (W64.of_int 0);
+    leakages <- LeakAddr([2]) :: leakages;
+    x.[2] <- aux_3;
+    leakages <- LeakFor(0,11) :: LeakAddr([]) :: leakages;
+    k <- 0;
+    while (k < 11) {
+      leakages <- LeakAddr([]) :: leakages;
+      aux_1 <- _P;
+      p <- aux_1;
+      leakages <- LeakAddr([]) :: leakages;
+      aux_2 <@ bN__muln_innerloop (x, k, 0, k, r, p);
+      x <- aux_2;
+      leakages <- LeakAddr([]) :: leakages;
+      aux_3 <- (W64.of_int 0);
+      zero <- aux_3;
+      leakages <- LeakAddr([k]) :: leakages;
+      aux_3 <- a.[k];
+      t0 <- aux_3;
+      leakages <- LeakAddr([]) :: leakages;
+      aux_2 <@ bN__addacc3 (x, zero, t0, k);
+      x <- aux_2;
+      leakages <- LeakAddr([(k %% 3)]) :: leakages;
+      aux_3 <- x.[(k %% 3)];
+      t0 <- aux_3;
+      leakages <- LeakAddr([]) :: leakages;
+      (aux_3, aux) <- mulu_64 t0 _U0;
+       _0 <- aux_3;
+      t0 <- aux;
+      leakages <- LeakAddr([]) :: leakages;
+      aux_3 <- t0;
+      leakages <- LeakAddr([k]) :: leakages;
+      r.[k] <- aux_3;
+      leakages <- LeakAddr([0]) :: leakages;
+      (aux_3, aux) <- mulu_64 t0 _P.[0];
+      t1 <- aux_3;
+      t0 <- aux;
+      leakages <- LeakAddr([]) :: leakages;
+      aux_2 <@ bN__addacc3 (x, t1, t0, k);
+      x <- aux_2;
+      k <- k + 1;
+    }
+    leakages <- LeakFor(11,((2 * 11) - 1)) :: LeakAddr([]) :: leakages;
+    aux_0 <- ((2 * 11) - 1);
+    k <- 11;
+    while (k < aux_0) {
+      leakages <- LeakAddr([]) :: leakages;
+      aux_1 <- _P;
+      p <- aux_1;
+      leakages <- LeakAddr([]) :: leakages;
+      aux_2 <@ bN__muln_innerloop (x, k, ((k - 11) + 1), 11, r, p);
+      x <- aux_2;
+      leakages <- LeakAddr([]) :: leakages;
+      aux_3 <- (W64.of_int 0);
+      zero <- aux_3;
+      leakages <- LeakAddr([k]) :: leakages;
+      aux_3 <- a.[k];
+      t0 <- aux_3;
+      leakages <- LeakAddr([]) :: leakages;
+      aux_2 <@ bN__addacc3 (x, zero, t0, k);
+      x <- aux_2;
+      leakages <- LeakAddr([(k %% 3)]) :: leakages;
+      aux_3 <- x.[(k %% 3)];
+      t0 <- aux_3;
+      leakages <- LeakAddr([]) :: leakages;
+      aux_3 <- t0;
+      leakages <- LeakAddr([(k - 11)]) :: leakages;
+      r.[(k - 11)] <- aux_3;
+      leakages <- LeakAddr([]) :: leakages;
+      aux_3 <- (W64.of_int 0);
+      leakages <- LeakAddr([(k %% 3)]) :: leakages;
+      x.[(k %% 3)] <- aux_3;
+      k <- k + 1;
+    }
+    leakages <- LeakAddr([]) :: leakages;
+    aux_3 <- (W64.of_int 0);
+    lastbit <- aux_3;
+    leakages <- LeakAddr([((2 * 11) - 1); (((2 * 11) - 1) %% 3)]) :: leakages;
+    (aux_4, aux_3) <- adc_64 x.[(((2 * 11) - 1) %% 3)] a.[((2 * 11) - 1)]
+    false;
+    cf <- aux_4;
+    leakages <- LeakAddr([(((2 * 11) - 1) %% 3)]) :: leakages;
+    x.[(((2 * 11) - 1) %% 3)] <- aux_3;
+    leakages <- LeakAddr([]) :: leakages;
+    (aux_4, aux_3) <- adc_64 lastbit (W64.of_int 0) cf;
+     _1 <- aux_4;
+    lastbit <- aux_3;
+    leakages <- LeakAddr([(((2 * 11) - 1) %% 3)]) :: leakages;
+    aux_3 <- x.[(((2 * 11) - 1) %% 3)];
+    leakages <- LeakAddr([(11 - 1)]) :: leakages;
+    r.[(11 - 1)] <- aux_3;
+    leakages <- LeakAddr([]) :: leakages;
+    aux_1 <- _mP;
+    mP <- aux_1;
+    leakages <- LeakAddr([]) :: leakages;
+    aux_1 <@ bN_cminusP_ (r, mP, lastbit);
+    r <- aux_1;
+    return (r);
+  }
+  
+  proc bN__pack2 (r:W64.t Array22.t, lo:W64.t Array11.t, hi:W64.t Array11.t) : 
+  W64.t Array22.t = {
+    var aux: int;
+    var aux_0: W64.t;
+    
+    var i:int;
+    var t:W64.t;
+    
+    leakages <- LeakFor(0,11) :: LeakAddr([]) :: leakages;
+    i <- 0;
+    while (i < 11) {
+      leakages <- LeakAddr([i]) :: leakages;
+      aux_0 <- lo.[i];
+      t <- aux_0;
+      leakages <- LeakAddr([]) :: leakages;
+      aux_0 <- t;
+      leakages <- LeakAddr([i]) :: leakages;
+      r.[i] <- aux_0;
+      i <- i + 1;
+    }
+    leakages <- LeakFor(0,11) :: LeakAddr([]) :: leakages;
+    i <- 0;
+    while (i < 11) {
+      leakages <- LeakAddr([i]) :: leakages;
+      aux_0 <- hi.[i];
+      t <- aux_0;
+      leakages <- LeakAddr([]) :: leakages;
+      aux_0 <- t;
+      leakages <- LeakAddr([(11 + i)]) :: leakages;
+      r.[(11 + i)] <- aux_0;
+      i <- i + 1;
+    }
+    return (r);
+  }
+  
+  proc bN_pack2_ (r:W64.t Array22.t, lo:W64.t Array11.t, hi:W64.t Array11.t) : 
+  W64.t Array22.t = {
+    var aux_0: W64.t Array11.t;
+    var aux: W64.t Array22.t;
+    
+    
+    
+    leakages <- LeakAddr([]) :: leakages;
+    aux <- r;
+    r <- aux;
+    leakages <- LeakAddr([]) :: leakages;
+    aux_0 <- lo;
+    lo <- aux_0;
+    leakages <- LeakAddr([]) :: leakages;
+    aux_0 <- hi;
+    hi <- aux_0;
+    leakages <- LeakAddr([]) :: leakages;
+    aux <@ bN__pack2 (r, lo, hi);
+    r <- aux;
+    leakages <- LeakAddr([]) :: leakages;
+    aux <- r;
+    r <- aux;
+    return (r);
+  }
+  
+  proc fPM_redM (r:W64.t Array11.t, a:W64.t Array22.t) : W64.t Array11.t = {
+    var aux: W64.t;
+    var aux_0: W64.t Array11.t;
+    
+    var _P0i:W64.t;
+    
+    leakages <- LeakAddr([]) :: leakages;
+    aux <- glob_P0i;
+    _P0i <- aux;
+    leakages <- LeakAddr([]) :: leakages;
+    aux_0 <@ bN__mont_redM (r, a, glob_P, glob_mP, _P0i);
+    r <- aux_0;
+    return (r);
+  }
+  
+  proc fPM_redM_ (r:W64.t Array11.t, a:W64.t Array22.t) : W64.t Array11.t = {
+    var aux: W64.t Array11.t;
+    var aux_0: W64.t Array22.t;
+    
+    
+    
+    leakages <- LeakAddr([]) :: leakages;
+    aux <- r;
+    r <- aux;
+    leakages <- LeakAddr([]) :: leakages;
+    aux_0 <- a;
+    a <- aux_0;
+    leakages <- LeakAddr([]) :: leakages;
+    aux <@ fPM_redM (r, a);
+    r <- aux;
+    leakages <- LeakAddr([]) :: leakages;
+    aux <- r;
+    r <- aux;
+    return (r);
+  }
+  
+  proc fPM_fromM_ (a:W64.t Array11.t) : W64.t Array11.t = {
+    var aux: W64.t Array11.t;
+    var aux_0: W64.t Array22.t;
+    
+    var _tmp:W64.t Array22.t;
+    var tmp2:W64.t Array11.t;
+    var tmp:W64.t Array22.t;
+    _tmp <- witness;
+    tmp <- witness;
+    tmp2 <- witness;
+    leakages <- LeakAddr([0]) :: leakages;
+    aux <- (Array11.init (fun i => _tmp.[0 + i]));
+    tmp2 <- aux;
+    leakages <- LeakAddr([]) :: leakages;
+    aux <@ bN_mov_ (tmp2, a);
+    tmp2 <- aux;
+    leakages <- LeakAddr([]) :: leakages;
+    aux <- tmp2;
+    leakages <- LeakAddr([0]) :: leakages;
+    _tmp <- Array22.init
+            (fun i => if 0 <= i < 0 + 11 then aux.[i-0] else _tmp.[i]);
+    leakages <- LeakAddr([11]) :: leakages;
+    aux <- (Array11.init (fun i => _tmp.[11 + i]));
+    tmp2 <- aux;
+    leakages <- LeakAddr([]) :: leakages;
+    aux <@ bN_set0_ (tmp2);
+    tmp2 <- aux;
+    leakages <- LeakAddr([]) :: leakages;
+    aux <- tmp2;
+    leakages <- LeakAddr([11]) :: leakages;
+    _tmp <- Array22.init
+            (fun i => if 11 <= i < 11 + 11 then aux.[i-11] else _tmp.[i]);
+    leakages <- LeakAddr([]) :: leakages;
+    aux_0 <- _tmp;
+    tmp <- aux_0;
+    leakages <- LeakAddr([]) :: leakages;
+    aux <@ fPM_redM_ (a, tmp);
+    a <- aux;
+    return (a);
+  }
+  
+  proc bN_rnd_ (a:W64.t Array11.t) : W64.t Array11.t = {
+    var aux_0: W8.t Array88.t;
+    var aux: W64.t Array11.t;
+    
+    
+    
+    leakages <- LeakAddr([]) :: leakages;
+    aux <- a;
+    a <- aux;
+    leakages <- LeakAddr([]) :: leakages;
+    aux_0 <@ SC.randombytes_88 ((Array88.init (fun i => get8
+                                (WArray88.init64 (fun i => (a).[i])) i)));
+    a <-
+    (Array11.init (fun i => get64 (WArray88.init8 (fun i => (aux_0).[i])) i));
+    leakages <- LeakAddr([]) :: leakages;
+    aux <- a;
+    a <- aux;
+    return (a);
+  }
+  
+  proc bN_rsample_ (a:W64.t Array11.t, bnd:W64.t Array11.t) : W64.t Array11.t = {
+    var aux_0: bool;
+    var aux: W64.t Array11.t;
+    
+    var cf:bool;
+    
+    leakages <- LeakAddr([]) :: leakages;
+    aux <@ bN_rnd_ (a);
+    a <- aux;
+    leakages <- LeakAddr([]) :: leakages;
+    aux_0 <@ bN_lt_cf_ (a, bnd);
+    cf <- aux_0;
+    leakages <- LeakCond((! cf)) :: LeakAddr([]) :: leakages;
+    
+    while ((! cf)) {
+      leakages <- LeakAddr([]) :: leakages;
+      aux <@ bN_rnd_ (a);
+      a <- aux;
+      leakages <- LeakAddr([]) :: leakages;
+      aux_0 <@ bN_lt_cf_ (a, bnd);
+      cf <- aux_0;
+    leakages <- LeakCond((! cf)) :: LeakAddr([]) :: leakages;
+    
+    }
+    return (a);
+  }
+  
+  proc fPM_chk_bnds_ (err:W64.t, a:W64.t Array11.t) : W64.t = {
+    var aux_0: bool;
+    var aux_1: W64.t;
+    var aux: W64.t Array11.t;
+    
+    var p:W64.t Array11.t;
+    var cf:bool;
+    var t:W64.t;
+    p <- witness;
+    leakages <- LeakAddr([]) :: leakages;
+    aux <- glob_P;
+    p <- aux;
+    leakages <- LeakAddr([]) :: leakages;
+    aux_0 <@ bN_lt_cf_ (a, p);
+    cf <- aux_0;
+    leakages <- LeakAddr([]) :: leakages;
+    aux_1 <@ bN__cf_mask (cf);
+    t <- aux_1;
+    leakages <- LeakAddr([]) :: leakages;
+    aux_1 <- NOT_64 t;
+    t <- aux_1;
+    leakages <- LeakAddr([]) :: leakages;
+    aux_1 <- (err `|` t);
+    err <- aux_1;
+    return (err);
+  }
+  
+  proc fPM_rnd_ (a:W64.t Array11.t) : W64.t Array11.t = {
+    var aux: W64.t Array11.t;
+    
+    var p:W64.t Array11.t;
+    p <- witness;
+    leakages <- LeakAddr([]) :: leakages;
+    aux <- glob_P;
+    p <- aux;
+    leakages <- LeakAddr([]) :: leakages;
+    aux <@ bN_rsample_ (a, p);
+    a <- aux;
+    return (a);
+  }
+  
+  proc fPM_addm_ (r:W64.t Array11.t, a:W64.t Array11.t, b:W64.t Array11.t) : 
+  W64.t Array11.t = {
+    var aux: bool;
+    var aux_1: W64.t;
+    var aux_0: W64.t Array11.t;
+    
+    var cf:bool;
+    var lastbit:W64.t;
+    var tmp:W64.t Array11.t;
+    var  _0:bool;
+    tmp <- witness;
+    leakages <- LeakAddr([]) :: leakages;
+    (aux, aux_0) <@ bN_add_ (r, a, b);
+    cf <- aux;
+    r <- aux_0;
+    leakages <- LeakAddr([]) :: leakages;
+    aux_1 <- (W64.of_int 0);
+    lastbit <- aux_1;
+    leakages <- LeakAddr([]) :: leakages;
+    (aux, aux_1) <- adc_64 lastbit (W64.of_int 0) cf;
+     _0 <- aux;
+    lastbit <- aux_1;
+    leakages <- LeakAddr([]) :: leakages;
+    aux_0 <- glob_mP;
+    tmp <- aux_0;
+    leakages <- LeakAddr([]) :: leakages;
+    aux_0 <@ bN_cminusP_ (r, tmp, lastbit);
+    r <- aux_0;
+    return (r);
+  }
+  
+  proc fPM_addmU_ (a:W64.t Array11.t, b:W64.t Array11.t) : W64.t Array11.t = {
+    var aux: bool;
+    var aux_1: W64.t;
+    var aux_0: W64.t Array11.t;
+    
+    var cf:bool;
+    var lastbit:W64.t;
+    var tmp:W64.t Array11.t;
+    var  _0:bool;
+    tmp <- witness;
+    leakages <- LeakAddr([]) :: leakages;
+    (aux, aux_0) <@ bN_addU_ (a, b);
+    cf <- aux;
+    a <- aux_0;
+    leakages <- LeakAddr([]) :: leakages;
+    aux_1 <- (W64.of_int 0);
+    lastbit <- aux_1;
+    leakages <- LeakAddr([]) :: leakages;
+    (aux, aux_1) <- adc_64 lastbit (W64.of_int 0) cf;
+     _0 <- aux;
+    lastbit <- aux_1;
+    leakages <- LeakAddr([]) :: leakages;
+    aux_0 <- glob_mP;
+    tmp <- aux_0;
+    leakages <- LeakAddr([]) :: leakages;
+    aux_0 <@ bN_cminusP_ (a, tmp, lastbit);
+    a <- aux_0;
+    return (a);
+  }
+  
+  proc fPM_subm_ (r:W64.t Array11.t, a:W64.t Array11.t, b:W64.t Array11.t) : 
+  W64.t Array11.t = {
+    var aux: bool;
+    var aux_0: W64.t Array11.t;
+    
+    var cf:bool;
+    var tmp:W64.t Array11.t;
+    tmp <- witness;
+    leakages <- LeakAddr([]) :: leakages;
+    (aux, aux_0) <@ bN_sub_ (r, a, b);
+    cf <- aux;
+    r <- aux_0;
+    leakages <- LeakAddr([]) :: leakages;
+    aux_0 <- glob_P;
+    tmp <- aux_0;
+    leakages <- LeakAddr([]) :: leakages;
+    aux_0 <@ bN_caddU_ (r, cf, tmp);
+    r <- aux_0;
+    return (r);
+  }
+  
+  proc fPM_submU_ (a:W64.t Array11.t, b:W64.t Array11.t) : W64.t Array11.t = {
+    var aux: bool;
+    var aux_0: W64.t Array11.t;
+    
+    var cf:bool;
+    var tmp:W64.t Array11.t;
+    tmp <- witness;
+    leakages <- LeakAddr([]) :: leakages;
+    (aux, aux_0) <@ bN_subU_ (a, b);
+    cf <- aux;
+    a <- aux_0;
+    leakages <- LeakAddr([]) :: leakages;
+    aux_0 <- glob_P;
+    tmp <- aux_0;
+    leakages <- LeakAddr([]) :: leakages;
+    aux_0 <@ bN_caddU_ (a, cf, tmp);
+    a <- aux_0;
+    return (a);
+  }
+  
+  proc fPM_mulm_ (r:W64.t Array11.t, a:W64.t Array11.t, b:W64.t Array11.t) : 
+  W64.t Array11.t = {
+    var aux_0: W64.t Array11.t;
+    var aux: W64.t Array22.t;
+    
+    var _tmp:W64.t Array22.t;
+    var tmp:W64.t Array22.t;
+    _tmp <- witness;
+    tmp <- witness;
+    leakages <- LeakAddr([]) :: leakages;
+    aux <- _tmp;
+    tmp <- aux;
+    leakages <- LeakAddr([]) :: leakages;
+    aux <@ bN_muln_ (tmp, a, b);
+    tmp <- aux;
+    leakages <- LeakAddr([]) :: leakages;
+    aux_0 <@ fPM_redM_ (r, tmp);
+    r <- aux_0;
+    return (r);
+  }
+  
+  proc fPM_mulmU_ (a:W64.t Array11.t, b:W64.t Array11.t) : W64.t Array11.t = {
+    var aux_0: W64.t Array11.t;
+    var aux: W64.t Array22.t;
+    
+    var _tmp:W64.t Array22.t;
+    var tmp:W64.t Array22.t;
+    _tmp <- witness;
+    tmp <- witness;
+    leakages <- LeakAddr([]) :: leakages;
+    aux <- _tmp;
+    tmp <- aux;
+    leakages <- LeakAddr([]) :: leakages;
+    aux <@ bN_muln_ (tmp, a, b);
+    tmp <- aux;
+    leakages <- LeakAddr([]) :: leakages;
+    aux_0 <@ fPM_redM_ (a, tmp);
+    a <- aux_0;
+    return (a);
+  }
+  
+  proc fPM_sqrm_ (r:W64.t Array11.t, a:W64.t Array11.t) : W64.t Array11.t = {
+    var aux_0: W64.t Array11.t;
+    var aux: W64.t Array22.t;
+    
+    var _tmp:W64.t Array22.t;
+    var tmp:W64.t Array22.t;
+    _tmp <- witness;
+    tmp <- witness;
+    leakages <- LeakAddr([]) :: leakages;
+    aux <- _tmp;
+    tmp <- aux;
+    leakages <- LeakAddr([]) :: leakages;
+    aux <@ bN_sqrn_ (tmp, a);
+    tmp <- aux;
+    leakages <- LeakAddr([]) :: leakages;
+    aux_0 <@ fPM_redM_ (r, tmp);
+    r <- aux_0;
+    return (r);
+  }
+  
+  proc fPM_sqrmU_ (a:W64.t Array11.t) : W64.t Array11.t = {
+    var aux_0: W64.t Array11.t;
+    var aux: W64.t Array22.t;
+    
+    var _tmp:W64.t Array22.t;
+    var tmp:W64.t Array22.t;
+    _tmp <- witness;
+    tmp <- witness;
+    leakages <- LeakAddr([]) :: leakages;
+    aux <- _tmp;
+    tmp <- aux;
+    leakages <- LeakAddr([]) :: leakages;
+    aux <@ bN_sqrn_ (tmp, a);
+    tmp <- aux;
+    leakages <- LeakAddr([]) :: leakages;
+    aux_0 <@ fPM_redM_ (a, tmp);
+    a <- aux_0;
+    return (a);
+  }
+  
+  proc fPM_expm_noct (r:W64.t Array11.t, a:W64.t Array11.t, b:W64.t Array11.t) : 
+  W64.t Array11.t = {
+    var aux_6: bool;
+    var aux_5: bool;
+    var aux_4: bool;
+    var aux_3: bool;
+    var aux_2: bool;
+    var aux_0: int;
+    var aux_1: W64.t;
+    var aux: W64.t Array11.t;
+    
+    var _b:W64.t Array11.t;
+    var _x:W64.t Array11.t;
+    var x:W64.t Array11.t;
+    var j:int;
+    var t:W64.t;
+    var _k:W64.t;
+    var zf:bool;
+    var cf:bool;
+    var  _0:bool;
+    var  _1:bool;
+    var  _2:bool;
+    var  _3:bool;
+    var  _4:bool;
+    var  _5:bool;
+    var  _6:bool;
+    _b <- witness;
+    _x <- witness;
+    x <- witness;
+    leakages <- LeakAddr([]) :: leakages;
+    aux <- b;
+    _b <- aux;
+    leakages <- LeakAddr([]) :: leakages;
+    aux <- _x;
+    x <- aux;
+    leakages <- LeakAddr([]) :: leakages;
+    aux <@ bN_mov_ (x, a);
+    x <- aux;
+    leakages <- LeakAddr([]) :: leakages;
+    aux <- x;
+    _x <- aux;
+    leakages <- LeakFor(0,11) :: LeakAddr([]) :: leakages;
+    j <- 0;
+    while (j < 11) {
+      leakages <- LeakAddr([]) :: leakages;
+      aux <- _b;
+      b <- aux;
+      leakages <- LeakAddr([j]) :: leakages;
+      aux_1 <- b.[j];
+      t <- aux_1;
+      leakages <- LeakAddr([]) :: leakages;
+      aux_1 <- (W64.of_int 64);
+      _k <- aux_1;
+      leakages <- LeakAddr([]) :: leakages;
+      (aux_6, aux_5, aux_4, aux_3, aux_2, aux_1) <- SHR_64 t (W8.of_int 1);
+       _0 <- aux_6;
+      cf <- aux_5;
+       _1 <- aux_4;
+       _2 <- aux_3;
+       _3 <- aux_2;
+      t <- aux_1;
+      leakages <- LeakAddr([]) :: leakages;
+      aux <- _x;
+      x <- aux;
+      leakages <- LeakCond(cf) :: LeakAddr([]) :: leakages;
+      if (cf) {
+        leakages <- LeakAddr([]) :: leakages;
+        aux <@ fPM_mulmU_ (r, x);
+        r <- aux;
+      } else {
+        
+      }
+      leakages <- LeakAddr([]) :: leakages;
+      aux <@ fPM_sqrmU_ (x);
+      x <- aux;
+      leakages <- LeakAddr([]) :: leakages;
+      aux <- x;
+      _x <- aux;
+      leakages <- LeakAddr([]) :: leakages;
+      (aux_6, aux_5, aux_4, aux_3, aux_1) <- DEC_64 _k;
+       _4 <- aux_6;
+       _5 <- aux_5;
+       _6 <- aux_4;
+      zf <- aux_3;
+      _k <- aux_1;
+      leakages <- LeakCond((! zf)) :: LeakAddr([]) :: leakages;
+      
+      while ((! zf)) {
+        leakages <- LeakAddr([]) :: leakages;
+        (aux_6, aux_5, aux_4, aux_3, aux_2, aux_1) <- SHR_64 t (W8.of_int 1);
+         _0 <- aux_6;
+        cf <- aux_5;
+         _1 <- aux_4;
+         _2 <- aux_3;
+         _3 <- aux_2;
+        t <- aux_1;
+        leakages <- LeakAddr([]) :: leakages;
+        aux <- _x;
+        x <- aux;
+        leakages <- LeakCond(cf) :: LeakAddr([]) :: leakages;
+        if (cf) {
+          leakages <- LeakAddr([]) :: leakages;
+          aux <@ fPM_mulmU_ (r, x);
+          r <- aux;
+        } else {
+          
+        }
+        leakages <- LeakAddr([]) :: leakages;
+        aux <@ fPM_sqrmU_ (x);
+        x <- aux;
+        leakages <- LeakAddr([]) :: leakages;
+        aux <- x;
+        _x <- aux;
+        leakages <- LeakAddr([]) :: leakages;
+        (aux_6, aux_5, aux_4, aux_3, aux_1) <- DEC_64 _k;
+         _4 <- aux_6;
+         _5 <- aux_5;
+         _6 <- aux_4;
+        zf <- aux_3;
+        _k <- aux_1;
+      leakages <- LeakCond((! zf)) :: LeakAddr([]) :: leakages;
+      
+      }
+      j <- j + 1;
+    }
+    return (r);
+  }
+  
+  proc fPM_expm_noct_ (r:W64.t Array11.t, a:W64.t Array11.t,
+                       b:W64.t Array11.t) : W64.t Array11.t = {
+    var aux: W64.t Array11.t;
+    
+    
+    
+    leakages <- LeakAddr([]) :: leakages;
+    aux <@ bN_mov_ (r, glob_exp0);
+    r <- aux;
+    leakages <- LeakAddr([]) :: leakages;
+    aux <- a;
+    a <- aux;
+    leakages <- LeakAddr([]) :: leakages;
+    aux <- b;
+    b <- aux;
+    leakages <- LeakAddr([]) :: leakages;
+    aux <@ fPM_expm_noct (r, a, b);
+    r <- aux;
+    leakages <- LeakAddr([]) :: leakages;
+    aux <- r;
+    r <- aux;
+    return (r);
+  }
+  
+  proc fPM_expmU_noct_ (a:W64.t Array11.t, b:W64.t Array11.t) : W64.t Array11.t = {
+    var aux: W64.t Array11.t;
+    
+    var _tmp:W64.t Array11.t;
+    var tmp:W64.t Array11.t;
+    _tmp <- witness;
+    tmp <- witness;
+    leakages <- LeakAddr([]) :: leakages;
+    aux <- _tmp;
+    tmp <- aux;
+    leakages <- LeakAddr([]) :: leakages;
+    aux <@ bN_mov_ (tmp, a);
+    tmp <- aux;
+    leakages <- LeakAddr([]) :: leakages;
+    aux <@ bN_mov_ (a, glob_exp0);
+    a <- aux;
+    leakages <- LeakAddr([]) :: leakages;
+    aux <@ fPM_expm_noct_ (a, tmp, b);
+    a <- aux;
+    return (a);
+  }
+  
+  proc fPM_expm (x0:W64.t Array11.t, x1:W64.t Array11.t, b:W64.t Array11.t) : 
+  W64.t Array11.t * W64.t Array11.t = {
+    var aux_6: bool;
+    var aux_5: bool;
+    var aux_4: bool;
+    var aux_3: bool;
+    var aux_2: bool;
+    var aux_0: int;
+    var aux_1: W64.t;
+    var aux_7: W64.t Array11.t;
+    var aux: W64.t Array11.t;
+    
+    var _b:W64.t Array11.t;
+    var j:int;
+    var t:W64.t;
+    var _k:W64.t;
+    var zf:bool;
+    var cf:bool;
+    var _t:W64.t;
+    var mask:W64.t;
+    var _mask:W64.t;
+    var  _0:bool;
+    var  _1:bool;
+    var  _2:bool;
+    var  _3:bool;
+    var  _4:bool;
+    var  _5:bool;
+    var  _6:bool;
+    _b <- witness;
+    leakages <- LeakAddr([]) :: leakages;
+    aux_7 <- b;
+    _b <- aux_7;
+    leakages <- LeakFor((- 1),(11 - 1)) :: LeakAddr([]) :: leakages;
+    aux_0 <- (11 - 1);
+    j <- (- 1);
+    while (aux_0 < j) {
+      leakages <- LeakAddr([]) :: leakages;
+      aux_7 <- _b;
+      b <- aux_7;
+      leakages <- LeakAddr([j]) :: leakages;
+      aux_1 <- b.[j];
+      t <- aux_1;
+      leakages <- LeakAddr([]) :: leakages;
+      aux_1 <- (W64.of_int 64);
+      _k <- aux_1;
+      leakages <- LeakAddr([]) :: leakages;
+      (aux_6, aux_5, aux_4, aux_3, aux_2, aux_1) <- SHL_64 t (W8.of_int 1);
+       _0 <- aux_6;
+      cf <- aux_5;
+       _1 <- aux_4;
+       _2 <- aux_3;
+       _3 <- aux_2;
+      t <- aux_1;
+      leakages <- LeakAddr([]) :: leakages;
+      aux_1 <- t;
+      _t <- aux_1;
+      leakages <- LeakAddr([]) :: leakages;
+      aux_1 <@ bN__cf_mask (cf);
+      mask <- aux_1;
+      leakages <- LeakAddr([]) :: leakages;
+      (aux_7, aux) <@ bN_cswap_mask_ (x0, x1, mask);
+      x0 <- aux_7;
+      x1 <- aux;
+      leakages <- LeakAddr([]) :: leakages;
+      aux_1 <- mask;
+      _mask <- aux_1;
+      leakages <- LeakAddr([]) :: leakages;
+      aux_7 <@ fPM_mulmU_ (x1, x0);
+      x1 <- aux_7;
+      leakages <- LeakAddr([]) :: leakages;
+      aux_7 <@ fPM_sqrmU_ (x0);
+      x0 <- aux_7;
+      leakages <- LeakAddr([]) :: leakages;
+      aux_1 <- _mask;
+      mask <- aux_1;
+      leakages <- LeakAddr([]) :: leakages;
+      (aux_7, aux) <@ bN_cswap_mask_ (x0, x1, mask);
+      x0 <- aux_7;
+      x1 <- aux;
+      leakages <- LeakAddr([]) :: leakages;
+      aux_1 <- _t;
+      t <- aux_1;
+      leakages <- LeakAddr([]) :: leakages;
+      (aux_6, aux_5, aux_4, aux_3, aux_1) <- DEC_64 _k;
+       _4 <- aux_6;
+       _5 <- aux_5;
+       _6 <- aux_4;
+      zf <- aux_3;
+      _k <- aux_1;
+      leakages <- LeakCond((! zf)) :: LeakAddr([]) :: leakages;
+      
+      while ((! zf)) {
+        leakages <- LeakAddr([]) :: leakages;
+        (aux_6, aux_5, aux_4, aux_3, aux_2, aux_1) <- SHL_64 t (W8.of_int 1);
+         _0 <- aux_6;
+        cf <- aux_5;
+         _1 <- aux_4;
+         _2 <- aux_3;
+         _3 <- aux_2;
+        t <- aux_1;
+        leakages <- LeakAddr([]) :: leakages;
+        aux_1 <- t;
+        _t <- aux_1;
+        leakages <- LeakAddr([]) :: leakages;
+        aux_1 <@ bN__cf_mask (cf);
+        mask <- aux_1;
+        leakages <- LeakAddr([]) :: leakages;
+        (aux_7, aux) <@ bN_cswap_mask_ (x0, x1, mask);
+        x0 <- aux_7;
+        x1 <- aux;
+        leakages <- LeakAddr([]) :: leakages;
+        aux_1 <- mask;
+        _mask <- aux_1;
+        leakages <- LeakAddr([]) :: leakages;
+        aux_7 <@ fPM_mulmU_ (x1, x0);
+        x1 <- aux_7;
+        leakages <- LeakAddr([]) :: leakages;
+        aux_7 <@ fPM_sqrmU_ (x0);
+        x0 <- aux_7;
+        leakages <- LeakAddr([]) :: leakages;
+        aux_1 <- _mask;
+        mask <- aux_1;
+        leakages <- LeakAddr([]) :: leakages;
+        (aux_7, aux) <@ bN_cswap_mask_ (x0, x1, mask);
+        x0 <- aux_7;
+        x1 <- aux;
+        leakages <- LeakAddr([]) :: leakages;
+        aux_1 <- _t;
+        t <- aux_1;
+        leakages <- LeakAddr([]) :: leakages;
+        (aux_6, aux_5, aux_4, aux_3, aux_1) <- DEC_64 _k;
+         _4 <- aux_6;
+         _5 <- aux_5;
+         _6 <- aux_4;
+        zf <- aux_3;
+        _k <- aux_1;
+      leakages <- LeakCond((! zf)) :: LeakAddr([]) :: leakages;
+      
+      }
+      j <- j - 1;
+    }
+    return (x0, x1);
+  }
+  
+  proc fPM_expm_ (x0:W64.t Array11.t, a:W64.t Array11.t, b:W64.t Array11.t) : 
+  W64.t Array11.t = {
+    var aux_0: W64.t Array11.t;
+    var aux: W64.t Array11.t;
+    
+    var _x1:W64.t Array11.t;
+    var x1:W64.t Array11.t;
+    var exp0:W64.t Array11.t;
+    var  _0:W64.t Array11.t;
+     _0 <- witness;
+    _x1 <- witness;
+    exp0 <- witness;
+    x1 <- witness;
+    leakages <- LeakAddr([]) :: leakages;
+    aux_0 <- _x1;
+    x1 <- aux_0;
+    leakages <- LeakAddr([]) :: leakages;
+    aux_0 <@ bN_mov_ (x1, a);
+    x1 <- aux_0;
+    leakages <- LeakAddr([]) :: leakages;
+    aux_0 <- glob_exp0;
+    exp0 <- aux_0;
+    leakages <- LeakAddr([]) :: leakages;
+    aux_0 <@ bN_mov_ (x0, exp0);
+    x0 <- aux_0;
+    leakages <- LeakAddr([]) :: leakages;
+    aux_0 <- b;
+    b <- aux_0;
+    leakages <- LeakAddr([]) :: leakages;
+    (aux_0, aux) <@ fPM_expm (x0, x1, b);
+    x0 <- aux_0;
+     _0 <- aux;
+    leakages <- LeakAddr([]) :: leakages;
+    aux_0 <- x0;
+    x0 <- aux_0;
+    return (x0);
+  }
+  
+  proc fPM_expmU_ (a:W64.t Array11.t, b:W64.t Array11.t) : W64.t Array11.t = {
+    var aux_0: W64.t Array11.t;
+    var aux: W64.t Array11.t;
+    
+    var _x1:W64.t Array11.t;
+    var x1:W64.t Array11.t;
+    var exp0:W64.t Array11.t;
+    var  _0:W64.t Array11.t;
+     _0 <- witness;
+    _x1 <- witness;
+    exp0 <- witness;
+    x1 <- witness;
+    leakages <- LeakAddr([]) :: leakages;
+    aux_0 <- _x1;
+    x1 <- aux_0;
+    leakages <- LeakAddr([]) :: leakages;
+    aux_0 <@ bN_mov_ (x1, a);
+    x1 <- aux_0;
+    leakages <- LeakAddr([]) :: leakages;
+    aux_0 <- glob_exp0;
+    exp0 <- aux_0;
+    leakages <- LeakAddr([]) :: leakages;
+    aux_0 <@ bN_mov_ (a, exp0);
+    a <- aux_0;
+    leakages <- LeakAddr([]) :: leakages;
+    aux_0 <- b;
+    b <- aux_0;
+    leakages <- LeakAddr([]) :: leakages;
+    (aux_0, aux) <@ fPM_expm (a, x1, b);
+    a <- aux_0;
+     _0 <- aux;
+    leakages <- LeakAddr([]) :: leakages;
+    aux_0 <- a;
+    a <- aux_0;
+    return (a);
+  }
+  
+  proc fPM_invmU_ (a:W64.t Array11.t) : W64.t Array11.t = {
+    var aux: W64.t Array11.t;
+    
+    var pm2:W64.t Array11.t;
+    pm2 <- witness;
+    leakages <- LeakAddr([]) :: leakages;
+    aux <- glob_Pm2;
+    pm2 <- aux;
+    leakages <- LeakAddr([]) :: leakages;
+    aux <@ fPM_expmU_noct_ (a, pm2);
+    a <- aux;
+    return (a);
+  }
+  
+  proc fPM_toM_ (a:W64.t Array11.t) : W64.t Array11.t = {
+    var aux: W64.t Array11.t;
+    
+    var rMP:W64.t Array11.t;
+    rMP <- witness;
+    leakages <- LeakAddr([]) :: leakages;
+    aux <- glob_rMP;
+    rMP <- aux;
+    leakages <- LeakAddr([]) :: leakages;
+    aux <@ fPM_mulmU_ (a, rMP);
+    a <- aux;
+    leakages <- LeakAddr([]) :: leakages;
+    aux <- a;
+    a <- aux;
+    return (a);
+  }
+}.
+
